mont_mul_add updates

impl/riscv/mont_mul_add_lemmas.i.dfy
@@ -27,24 +27,180 @@ module mont_mul_add_lemmas {
     r := refine_uint64_view(0, 0, 0);
   }
   
-  predicate mont_mul_add_loop_inv(
-    A: uint64_view_t,
-    B: uint64_view_t,
-    A_prev: uint64_view_t,
-    B_prev: uint64_view_t,
-    n: seq<uint32>,
-    b: seq<uint32>,
-    c: seq<uint32>,
-    a: uint32,
-    d0: uint32,
-    i: nat)
-  {
-    && |n| == |b| == |c|
-    && 0 <= i < |n|
+ //  predicate mont_mul_add_loop_inv(
+ //    A: uint64_view_t,
+ //    B: uint64_view_t,
+ //    A_prev: uint64_view_t,
+ //    B_prev: uint64_view_t,
+ //    n: seq<uint32>,
+ //    b: seq<uint32>,
+ //    c: seq<uint32>,
+ //    a: uint32,
+ //    d0: uint32,
+ //    i: nat)
+ //  {
+ //    && |n| == |b| == |c|
+ //    && 0 <= i < |n|
 
-    && A.full == a * b[i] + c[i] + A_prev.uh
-    && B.full == d0 * n[i] + A.lh + B_prev.uh
-    && (i > 0 ==> c[i-1] == B.lh)
-  }
+ //    && A.full == a * b[i] + c[i] + A_prev.uh
+ //    && B.full == d0 * n[i] + A.lh + B_prev.uh
+ //    && (i > 0 ==> c[i-1] == B.lh)
+ //  }
+
+    lemma mont_loop_cong_lemma(
+        p1: uint64_view_t,
+        a0: uint32,
+        y0: uint32,
+        xi: uint32,
+        w25: uint32,
+        w26: uint32,
+        m0d: uint32)
+
+        requires a0 + y0 * xi == p1.full;
+        requires ToNat([w25, w26]) == p1.lh * m0d; 
+        ensures cong_B32(w25, (a0 + y0 * xi) * m0d);
+    {
+        calc ==> {
+            true;
+            cong_B32(a0 + y0 * xi, p1.full);
+                { uint64_view_lemma(p1); }
+            cong_B32(a0 + y0 * xi, p1.lh + p1.uh * BASE_32);
+            cong_B32(a0 + y0 * xi, p1.lh);
+            cong_B32(p1.lh, a0 + y0 * xi);
+                { LemmaModMulEquivalentAuto(); }
+            cong_B32(p1.lh * m0d, (a0 + y0 * xi) * m0d);
+        }
+
+        calc ==> {
+            true;
+                { LemmaSeqLen2([w25, w26]); }
+            w25 + w26 * BASE_32 == p1.lh * m0d;
+            cong_B32(w25 + w26 * BASE_32, p1.lh * m0d);
+            cong_B32(w25 + w26 * BASE_32, (a0 + y0 * xi) * m0d);
+            cong_B32(w25, (a0 + y0 * xi) * m0d);
+        }
+    }
+
+    lemma mont_loop_divisible_lemma(
+        ui: int,
+        m0d: int,
+        p1: uint64_view_t,
+        p2: uint64_view_t,
+        m0: int)
+
+        requires p2.full == ui * m0 + p1.lh;
+        requires cong_B32(m0d * m0, -1);
+        requires cong_B32(ui, p1.full * m0d);
+        ensures p2.lh == 0;
+    {
+        var p1_full := p1.full as int;
+
+        assert cong_B32(ui * m0, -p1_full) by {
+            assert cong_B32(m0d * m0 * p1.full, -p1_full) by {
+                LemmaModMulEquivalent(m0d * m0, -1, p1.full, BASE_32);
+            }
+            assert cong_B32(ui * m0, p1.full * m0d * m0) by {
+                LemmaModMulEquivalentAuto();
+            }
+            assert p1.full * m0d * m0 == m0d * m0 * p1.full by {
+                LemmaMulIsAssociativeAuto();
+            }
+        }
+
+        calc ==> {
+            cong_B32(ui * m0, -p1_full);
+            cong_B32(ui * m0 + p1.lh , - p1_full + p1.lh);
+                { lemma_uint64_half_split(p1.full); }
+            cong_B32(ui * m0 + p1.lh, - (p1.uh as int * BASE_32 + p1.lh) + p1.lh);
+            cong_B32(ui * m0 + p1.lh, - (p1.uh as int) * BASE_32);
+                { assert cong_B32(- (p1.uh as int) * BASE_32, 0); }
+            cong_B32(ui * m0 + p1.lh, 0);
+        }
+
+        calc ==> {
+            p2.full == ui * m0 + p1.lh;
+                { lemma_uint64_half_split(p2.full); }
+            p2.lh + p2.uh * BASE_32 == ui * m0 + p1.lh;
+            cong_B32(p2.lh + p2.uh * BASE_32, ui * m0 + p1.lh);
+            cong_B32(ui * m0 + p1.lh, p2.lh + p2.uh * BASE_32);
+            cong_B32(ui * m0 + p1.lh, p2.lh);
+            cong_B32(p2.lh, 0);
+        }
+
+        assert cong_B32(p2.lh, 0);
+    }
+
+    predicate mont_loop_inv(
+        xi: uint32,
+        ui: uint32,
+        p1: uint512_view_t,
+        p2: uint512_view_t,
+        y: seq<uint32>,
+        m: seq<uint32>,
+        prev_a: seq<uint32>,
+        next_a: seq<uint32>,
+        j: nat)
+    {
+        && |m| == |next_a| == |y| == |prev_a| == NUM_WORDS
+        && (1 <= j <= NUM_WORDS)
+        && (xi * ToNat(y[..j]) + ui * ToNat(m[..j]) + ToNat(prev_a[..j]) 
+            == 
+        ToNat([0] + next_a[..j-1]) + p2.uh * pow_B32(j) + p1.uh * pow_B32(j))
+    }
+
+
+    lemma mont_loop_inv_pre_lemma(
+        xi: uint32, // a
+        ui: uint32, //d0
+        m0d: uint32, //d0inv
+        p1: uint64_view_t, // A
+        p2: uint64_view_t, // B
+        y: seq<uint32>, // b
+        m: seq<uint32>, // n
+        a: seq<uint32>) // c
+        requires |m| == |a| == |y| == NUM_WORDS;
+        requires p1.full == xi * y[0] + a[0]; // A
+        requires p2.full == ui * m[0] + p1.lh; // B == d0 * n[0] + A.lh
+        requires cong_B32(m0d * ToNat(m), -1);
+        requires cong_B32(ui, (a[0] + y[0] * xi) * m0d);
+
+        ensures mont_loop_inv(xi, ui, p1, p2, y, m, a, a, 1)
+    {
+        assert cong_B32(m0d * m[0], -1) by {
+            LemmaSeqLswModEquivalence(m);
+            LemmaModMulEquivalent(ToNat(m), m[0], m0d, BASE_32);
+            LemmaMulIsCommutativeAuto();
+        }
+
+        mont_loop_divisible_lemma(ui, m0d, p1, p2, m[0]);
+
+        LemmaSeqLen1(y[..1]);
+        LemmaSeqLen1(m[..1]);
+        LemmaSeqLen1(a[..1]);
+
+        assert p2.full == p2.uh * BASE_32 by {
+            uint64_view_lemma(p2);
+        }
+
+        uint64_view_lemma(p1);
+
+        calc {
+            xi * ToNat(y[..1]) + ui * ToNat(m[..1]) + ToNat(a[..1]);
+                { reveal Pow(); }
+            p2.uh * pow_B32(1) + p1.uh * pow_B32(1);
+                {
+                    reveal ToNatRight();
+                    assert ToNat([0]) == 0;
+                }
+            ToNat([0]) + p2.uh * pow_B32(1) + p1.uh * pow_B32(1);
+                {
+                    assert [0] + a[..0] == [0];
+                    assert ToNat([0]) == ToNat([0] + a[..0]);
+                }
+            ToNat([0] + a[..0]) + p2.uh * pow_B32(1) + p1.uh * pow_B32(1);
+
+        }
+    }
+
 
 }
